theories/sim/invariant.v
@@ -71,7 +71,8 @@ Definition lmap_inv (r: resUR) (σs σt: state) : Prop :=
   ∀ (l: loc), l ∈ dom (gset loc) r.(rlm) → l ∈ dom (gset loc) σt.(shp) ∧
     ∀ s stk,
     r.(rlm) !! l ≡ Some (to_locStateR (lsLocal s stk)) →
-    σs.(shp) !! l = Some s ∧ σt.(shp) !! l = Some s.
+    σs.(shp) !! l = Some s ∧ σt.(shp) !! l = Some s ∧
+    σs.(sst) !! l = Some stk ∧ σt.(sst) !! l = Some stk.
 
 (* [l] is private w.r.t to some tag [t] if [t] is uniquely owned and protected
   by some call id [c] and [l] is in [t]'s heaplet [h]. *)
